logand as sum

code/ecdsa/Hacl.Impl.EC.Masking.ScalarAccess.fst
@@ -1,12 +1,12 @@
 module Hacl.Impl.EC.Masking.ScalarAccess
 
-
 open FStar.HyperStack.All
 open FStar.HyperStack
 module ST = FStar.HyperStack.ST
 
 open Lib.IntTypes
 open Lib.Buffer
+open Lib.ByteBuffer
 open Lib.Loops
 
 open Spec.ECC
@@ -16,11 +16,13 @@ open Hacl.Impl.EC.Masking
 open Hacl.Spec.EC.Definition
 open Hacl.Impl.EC.PointDouble
 
+open FStar.Mul
 
-#set-options " --z3rlimit 200"
+module BV = FStar.BitVector
 
 
-inline_for_extraction noextract
+#set-options "--fuel 0 --ifuel 0 --z3rlimit 200"
+
 val getScalarBit_leftEndian: #c: curve 
   -> #buf_type: buftype 
   -> s:lbuffer_t buf_type uint8 (getScalarLenBytes c) 
@@ -43,52 +45,211 @@ val getScalarBit_l: #c: curve
   -> n:size_t{v n < v (getScalarLen c)}
   -> Stack uint64
     (requires fun h0 -> live h0 s)
-    (ensures  fun h0 r h1 -> h0 == h1 /\ r == ith_bit #c (as_seq h0 s) (v n) /\ v r <= 1)
+    (ensures  fun h0 r h1 -> modifies0 h0 h1 /\ r == ith_bit #c (as_seq h0 s) (v n) /\ v r <= 1)
 
 let getScalarBit_l #c #b s n = 
   push_frame();
-    let h0 = ST.get() in 
     let temp = create (size 1) (u64 0) in 
-    let inv h i = modifies (loc temp) h0 h /\ live h temp in 
-    for 0ul (getScalarLen c) inv (fun i -> 
-      let bit = getScalarBit_leftEndian s n in 
-      assert(bit == ith_bit (as_seq h0 s) (v n));
+    let h0 = ST.get() in 
+    let inv h i = modifies (loc temp) h0 h /\ live h0 temp /\ (
+      let temp0 = Lib.Sequence.index (as_seq h temp) 0 in v temp0 <= 1 /\ (
+      if i > v n then v temp0 == v (ith_bit (as_seq h0 s) (v n)) else True)) in 
+
+  for 0ul (getScalarLen c) inv (fun i -> 
+    let h0_ = ST.get() in 
+    
+    let bit = getScalarBit_leftEndian s n in 
+    assert(bit == ith_bit (as_seq h0 s) (v n));
       
-      let mask = neq_mask (size_to_uint64 n) (size_to_uint64 i) in 
-	neq_mask_lemma (size_to_uint64 n) (size_to_uint64 i);
-      copy_conditional_u64 bit temp mask);
+    let mask = eq_mask (size_to_uint64 n) (size_to_uint64 i) in 
+      eq_mask_lemma (size_to_uint64 n) (size_to_uint64 i);
+    copy_conditional_u64 bit temp mask
+  );
+
   let result = index temp (size 0) in
-  admit();
+  let h1 = ST.get() in 
   pop_frame();
   result
-    
 
-[@ CInline]
-inline_for_extraction noextract  
-val getScalar_4: #buf_type: buftype 
-  -> scalar: lbuffer_t buf_type uint8 (size 32) -> i: size_t {v i < 64} -> 
-  Stack uint32 
-    (requires fun h -> live h scalar)
-    (ensures fun h0 _ h1 -> True)
+
+inline_for_extraction noextract
+val get_high_part: a:uint64 -> r:uint32{uint_v r == uint_v a / pow2 32}
+let get_high_part a = to_u32 (shift_right a (size 32))
+
+inline_for_extraction noextract
+val get_low_part: a:uint64 -> r:uint32{uint_v r == uint_v a % pow2 32}
+let get_low_part a = to_u32 a
+
+val append_uint: #n1:nat -> #n2:nat
+  -> num1:UInt.uint_t n1 -> num2:UInt.uint_t n2 -> UInt.uint_t (n1 + n2)
+
+val shift_bound: #n:nat -> num:UInt.uint_t n -> n':nat ->
+  Lemma (num * pow2 n' <= pow2 (n' + n) - pow2 n')
+
+let shift_bound #n num n' =
+  Math.Lemmas.lemma_mult_le_right (pow2 n') num (pow2 n - 1);
+  Math.Lemmas.distributivity_sub_left (pow2 n) 1 (pow2 n');
+  Math.Lemmas.pow2_plus n' n
+
+
+let append_uint #n1 #n2 num1 num2 =
+  shift_bound num2 n1;
+  num1 + num2 * pow2 n1
+
+val to_vec_append : #n1:pos-> #n2:pos -> num1:UInt.uint_t n1 -> num2:UInt.uint_t n2 ->
+  Lemma (UInt.to_vec (append_uint num1 num2) ==
+         Seq.append (UInt.to_vec num2) (UInt.to_vec num1))
+
+let to_vec_append #n1 #n2 num1 num2 =
+  UInt.append_lemma (UInt.to_vec num2) (UInt.to_vec num1)
+
+val to_vec_low_high: a:UInt.uint_t 64 -> Lemma
+  (UInt.to_vec a ==
+   Seq.append (UInt.to_vec #32 (a / pow2 32)) (UInt.to_vec #32 (a % pow2 32)))
+
+let to_vec_low_high a =
+  assert (a == append_uint #32 #32 (a % pow2 32) (a / pow2 32));
+  to_vec_append #32 #32 (a % pow2 32) (a / pow2 32)
+
+
+val logand_vec_append (#n1 #n2: pos) (a1 b1: BV.bv_t n1) (a2 b2: BV.bv_t n2) :
+  Lemma (Seq.append (BV.logand_vec a1 b1) (BV.logand_vec a2 b2) ==
+         BV.logand_vec #(n1 + n2) (FStar.Seq.append a1 a2) (FStar.Seq.append b1 b2))
+
+let logand_vec_append #n1 #n2 a1 b1 a2 b2 =
+  Seq.lemma_eq_intro (Seq.append (BV.logand_vec a1 b1) (BV.logand_vec a2 b2))
+                     (BV.logand_vec #(n1 + n2) (Seq.append a1 a2) (Seq.append b1 b2))
+
+val lemma_and_both_parts: a: uint64 -> b: uint64 -> Lemma (
+  let a0, a1 = get_low_part a, get_high_part a in 
+  let b0, b1 = get_low_part b, get_high_part b in 
+  v (logand a1 b1) * pow2 32 + v (logand a0 b0) == v (logand a b))
+
+let lemma_and_both_parts a b = 
+  to_vec_low_high (v a);
+  to_vec_low_high (v b);
+    let a0, a1 = get_low_part a, get_high_part a in 
+    let b0, b1 = get_low_part b, get_high_part b in 
+
+
+  let a0_ = UInt.to_vec #32 (v a0) in
+  let a1_ = UInt.to_vec #32 (v a1) in
+
+
+  let b0_ = UInt.to_vec #32 (v b0) in
+  let b1_ = UInt.to_vec #32 (v b1) in
+  
+  assert(UInt.to_vec #64 (v a) == Seq.append a1_ a0_);
+  assert(UInt.to_vec #64 (v b) == Seq.append b1_ b0_);
+  
+
+  logand_vec_append a1_ b1_ a0_ b0_;
+
+  assert(Seq.append (BV.logand_vec a1_ b1_) (BV.logand_vec a0_ b0_) ==
+         BV.logand_vec #64  (FStar.Seq.append a1_ a0_) (FStar.Seq.append b1_ b0_));
+
+  UInt.append_lemma a1_ a0_;
+  UInt.append_lemma b1_ b0_;
+  assert( (Seq.append a1_ a0_) == UInt.to_vec #64 (v a));
+  assert(UInt.from_vec #64 (Seq.append b1_ b0_) == v b);
+
+
+  assert( (Seq.append (BV.logand_vec a1_ b1_) (BV.logand_vec a0_ b0_)) ==
+          (BV.logand_vec #64 (UInt.to_vec #64 (v a)) (UInt.to_vec #64 (v b))));
+
+
+  logand_spec a b;
+  assert(UInt.from_vec (BV.logand_vec #64 (UInt.to_vec #64 (v a)) (UInt.to_vec #64 (v b))) == v (logand a b));
+  
+  logand_spec a1 b1;
+  assert(UInt.from_vec (BV.logand_vec #32 (UInt.to_vec #32 (v a1)) (UInt.to_vec #32 (v b1))) == v (logand a1 b1));
+  logand_spec a0 b0;
+  assert(UInt.from_vec (BV.logand_vec #32 (UInt.to_vec #32 (v a0)) (UInt.to_vec #32 (v b0))) == v (logand a0 b0));
+  
+
+  UInt.append_lemma (BV.logand_vec a1_ b1_) (BV.logand_vec a0_ b0_);
+  assert(v (logand a1 b1) * pow2 32 + v (logand a0 b0) == v (logand a b))
+
+
+
+val getScalar_4: #c: curve
+  -> #buf_type: buftype 
+  -> s: scalar_t #buf_type #c
+  -> i: size_t {v i < v (getScalarLenBytes c) * 2} -> 
+  Stack uint32
+  (requires fun h -> live h s)
+  (ensures fun h0 r h1 -> 
+    let radix = 4 in 
+    let s = as_seq h0 s in 
+    v r == FStar.Math.Lib.arithmetic_shift_right (scalar_as_nat #c s) (radix * v i) % pow2 radix)
 
 let getScalar_4 #a scalar i = 
+  let h0 = ST.get() in
+  
   let half = shift_right i 1ul in 
     shift_right_lemma i 1ul;
   let word = to_u32 (index scalar half) in 
-  let bitShift : size_t = logand i (size 1) in 
+  let bitShift = logand i (size 1) in 
     logand_mask i (size 1) 1; 
   let bitShiftAsPrivate = size_to_uint32 bitShift in 
-  let mask : uint32 = cmovznz01 (u32 0xf0) (u32 0x0f) bitShiftAsPrivate in  
+  
+  let mask = cmovznz01 (u32 0xf0) (u32 0x0f) bitShiftAsPrivate in  
   let shiftMask = cmovznz01 (size 0x4) (size 0x0) bitShift in
-  let result : uint32 = logand word mask in 
-  let result : uint32 = shift_right result shiftMask in 
+  
+  let result0 = logand word mask in 
+  let result = shift_right result0 shiftMask in 
+
+  let index = v i in 
+  assert(v half = index / 2);
+  assert(v word = v (Lib.Sequence.index (as_seq h0 scalar) (index / 2)));
+  
+  assert(if index % 2 = 0 then v mask = 0xf0 else v mask = 0x0f);
+  assert(if index % 2 = 0 then v shiftMask = 4 else v shiftMask = 0);
+
+  if index % 2 = 0 then 
+    begin
+      logand_spec word mask;
+      assert(v result0 = logand_v (v word) (v mask));
+      assert(v mask = 0xf0);
+      assert(v result = v result0 / pow2 4)
+    end
+  else
+    begin
+      assert(v mask = 0x0f);
+      logand_mask word mask 4;
+      assert(v result0 = v word % pow2 4);
+      assert(v result = v (Lib.Sequence.index (as_seq h0 scalar) (index / 2)) % pow2 4)
+    end;
+
+  admit();
   result
+
+
+inline_for_extraction noextract
+val getScalar_4_byBit: #c: curve
+  -> #buf_type: buftype 
+  -> s: scalar_t #buf_type #c
+  -> i: size_t {v i < v (getScalarLenBytes c) * 2} -> 
+  Stack uint64
+    (requires fun h -> live h s)
+    (ensures fun h0 _ h1 -> True)
+
+
+let getScalar_4_byBit #c s i = 
+  let bit = getScalarLen c -! 1ul -! (shift_left i 2ul) in 
+  
+  let bit0 = shift_left (getScalarBit_leftEndian s bit) 3ul in 
+  let bit1 = shift_left (getScalarBit_leftEndian s (bit -! 1ul)) 2ul in 
+  let bit2 = shift_left (getScalarBit_leftEndian s (bit -! 2ul)) 1ul in 
+  let bit3 = shift_left (getScalarBit_leftEndian s (bit -! 3ul)) 0ul in 
+  logxor (logxor bit0 bit1) (logxor bit2 bit3)
+
 
 
 open Hacl.Impl.EC.Precomputed
 
 inline_for_extraction noextract
-val getPointPrecomputedMixed_: #c: curve -> scalar: lbuffer uint8 (size 32) -> 
+val getPointPrecomputedMixed_: #c: curve -> scalar: scalar_t #MUT #c -> 
   i:size_t{v i < 64} -> pointToAdd: lbuffer uint64 (size 8) ->
   Stack unit 
   (requires fun h -> live h scalar /\ live h pointToAdd)
@@ -96,7 +257,9 @@ val getPointPrecomputedMixed_: #c: curve -> scalar: lbuffer uint8 (size 32) ->
 
 let getPointPrecomputedMixed_ #c scalar i pointToAdd = 
   push_frame();
-    let bits: uint32 = getScalar_4 scalar i in
+    let bits = getScalar_4_byBit scalar i in 
+  (*   let r =  shift_right (to_u64 bits) 18ul in 
+    let bits = getScalar_4 #c scalar i in *)
     let invK h (k: nat) = True in 
     Lib.Loops.for 0ul 16ul invK
     (fun k -> 
