code/ecdsa/Hacl.Impl.EC.Core.fst
@@ -570,9 +570,9 @@ val secretToPublic_0: #c: curve -> #t: buftype -> q: point c -> result: point c 
 
 
 let secretToPublic_0 #c q result scalar tempBuffer = 
-  uploadStartPointsS2P q result; 
+  (* uploadStartPointsS2P q result;  *)
 (*   montgomery_ladder q result scalar tempBuffer *)
-  Hacl.Impl.EC.Masking.ScalarAccess.montgomery_ladder_2_precomputed result scalar tempBuffer;
+  Hacl.Impl.EC.ScalarMult.Radix.montgomery_ladder_2_precomputed result scalar tempBuffer;
   copy q result
 
 
